src/spec/TLS13.ConnectionState.ProtectedWireLemmas.fsti
@@ -876,6 +876,80 @@ val lemma_conn_events_received_decode_replay_append_split
             suffix_received
             final_model)
 
+val lemma_sent_received_replay_append_split_equal_tails
+  (sender_model:CS.connection_model)
+  (receiver_model:CS.connection_model)
+  (sender_prefix:list CS.conn_event)
+  (sender_suffix:list CS.conn_event)
+  (receiver_prefix:list CS.conn_event)
+  (receiver_suffix:list CS.conn_event)
+  (sender_raw_sent:B.bytes)
+  (sender_raw_received:B.bytes)
+  (receiver_raw_sent:B.bytes)
+  (receiver_raw_received:B.bytes)
+  (sender_final:CS.connection_model)
+  (receiver_final:CS.connection_model)
+  : Lemma
+      (requires
+        CS.conn_events_sent_seal_replay
+          sender_model
+          (FStar.List.Tot.append sender_prefix sender_suffix)
+          sender_raw_sent
+          sender_raw_received
+          sender_final /\
+        CS.conn_events_received_decode_replay
+          receiver_model
+          (FStar.List.Tot.append receiver_prefix receiver_suffix)
+          receiver_raw_sent
+          receiver_raw_received
+          receiver_final /\
+        Seq.equal sender_raw_sent receiver_raw_received)
+      (ensures
+        exists sender_mid receiver_mid
+          sender_prefix_sent sender_prefix_received
+          sender_suffix_sent sender_suffix_received
+          receiver_prefix_sent receiver_prefix_received
+          receiver_suffix_sent receiver_suffix_received.
+          Seq.equal
+            sender_raw_sent
+            (B.append sender_prefix_sent sender_suffix_sent) /\
+          Seq.equal
+            sender_raw_received
+            (B.append sender_prefix_received sender_suffix_received) /\
+          Seq.equal
+            receiver_raw_sent
+            (B.append receiver_prefix_sent receiver_suffix_sent) /\
+          Seq.equal
+            receiver_raw_received
+            (B.append receiver_prefix_received receiver_suffix_received) /\
+          CS.conn_events_sent_seal_replay
+            sender_model
+            sender_prefix
+            sender_prefix_sent
+            sender_prefix_received
+            sender_mid /\
+          CS.conn_events_sent_seal_replay
+            sender_mid
+            sender_suffix
+            sender_suffix_sent
+            sender_suffix_received
+            sender_final /\
+          CS.conn_events_received_decode_replay
+            receiver_model
+            receiver_prefix
+            receiver_prefix_sent
+            receiver_prefix_received
+            receiver_mid /\
+          CS.conn_events_received_decode_replay
+            receiver_mid
+            receiver_suffix
+            receiver_suffix_sent
+            receiver_suffix_received
+            receiver_final /\
+          (Seq.length sender_prefix_sent ==
+             Seq.length receiver_prefix_received ==>
+           Seq.equal sender_suffix_sent receiver_suffix_received))
+
 val lemma_step_received_network_event_preserves_record_write
   (model:CS.connection_model)
   (msg:M.tls_message)
